\documentclass[12pt,a4paper]{article}
\author{Adheesh Juvekar, Arul Thileeban}

\usepackage{amsfonts}
\usepackage[left=10mm,top=20mm,right=10mm,bottom=20mm]{geometry}

\hbadness=99999

\begin{document}
\title{Homework 1}
\maketitle

\section*{Written Problems}
\begin{enumerate}
    \item 
    $\hat{\pi}_0 = \frac{1}{\left| \cal D \right|}\sum_{i\in\cal D}{\mathbb{I}(y_i = 0)}$\\
    $\hat{\pi}_0 = \frac{1}{10} \times 5$\\
    $\hat{\pi}_0 = 0.5$\\\\
    $\hat{\pi}_1 = \frac{1}{\left| \cal D \right|}\sum_{i\in\cal D}{\mathbb{I}(y_i = 1)}$\\
    $\hat{\pi}_1 = \frac{1}{10} \times 5$\\
    $\hat{\pi}_1 = 0.5$\\\\
    $H\left(\hat{\pi}\right) = -\left( \sum_{c=0}^{1}{\hat{\pi_c}log_e\hat{\pi_c}} \right) $\\
    $H\left(\hat{\pi}\right) = -\left( 0.5 \times log_e0.5 + 0.5 \times log_e0.5 \right)$\\
    $H\left(\hat{\pi}\right) = -\left( -0.6931 \right)$\\
    $H\left(\hat{\pi}\right) = 0.6931$\\\\
    $InfoGain(X_1) = H\left( \hat{\pi} \right)-H\left(\ \hat{\pi} | X_1 \right)$\\
    $InfoGain(X_1) = 0.6931 - \left[ \left( -\frac{8}{10}\times\left( \frac{5}{8}\times log_e(\frac{5}{8})+\frac{3}{8}\times log_e(\frac{3}{8}) \right) \right)+ \left( -\frac{2}{10}\times\left( 0+1\times log_e(1) \right) \right) \right] $\\
	$InfoGain(X_1) = 0.6931 - \left[ 0.5292 + 0 \right]$\\
	$InfoGain(X_1) = 0.1639$\\\\
	 
    $InfoGain(X_2) = H\left( \hat{\pi} \right)-H\left(\ \hat{\pi} | X_2 \right)$\\
    $InfoGain(X_2) = 0.6931 - \left[ \left( -\frac{6}{10}\times\left( \frac{4}{6}\times log_e(\frac{4}{6})+\frac{2}{6}\times log_e(\frac{2}{6}) \right) \right)+ \left( -\frac{4}{10}\times\left( \frac{1}{4}\times log_e(\frac{1}{4})+\frac{3}{4}\times log_e(\frac{3}{4}) \right) \right) \right] $\\
	$InfoGain(X_2) = 0.6931 - \left[ 0.3819 + 0.2249 \right]$\\
	$InfoGain(X_2) = 0.0863$\\\\
	
	$InfoGain(X_3) = H\left( \hat{\pi} \right)-H\left(\ \hat{\pi} | X_3 \right)$\\
	$InfoGain(X_3) = 0.6931 - \left[ \left( -\frac{6}{10}\times\left( \frac{3}{6}\times log_e(\frac{3}{6})+\frac{3}{6}\times log_e(\frac{3}{6}) \right) \right)+ \left( -\frac{4}{10}\times\left( \frac{2}{4}\times log_e(\frac{2}{4})+\frac{2}{4}\times log_e(\frac{2}{4}) \right) \right) \right] $\\
	$InfoGain(X_3) = 0.6931 - \left[ 0.6931 \right]$\\
	$InfoGain(X_3) = 0$\\\\
	
	$InfoGain(X_4) = H\left( \hat{\pi} \right)-H\left(\ \hat{\pi} | X_4 \right)$\\
	$InfoGain(X_4) = 0.6931 - \left[ \left( -\frac{5}{10}\times\left( \frac{3}{5}\times log_e(\frac{3}{5})+\frac{2}{5}\times log_e(\frac{2}{5}) \right) \right)+ \left( -\frac{5}{10}\times\left( \frac{2}{5}\times log_e(\frac{2}{5})+\frac{3}{5}\times log_e(\frac{3}{5}) \right) \right) \right] $\\
	$InfoGain(X_4) = 0.6931 - \left[ 0.3365 + 0.3365 \right]$\\
	$InfoGain(X_4) = 0.0201$\\\\
	
	Therefore, $InfoGain(X_1) > InfoGain(X_2)>InfoGain(X_4)>InfoGain(X_3)$\\
	Hence, \textbf{Decision tree algorithm will choose $X_1$ for the first split of the following dataset.}\\
	
	\item
	\begin{enumerate}

	    \item 
	    $p(D/ \theta) = \theta^{N_1} {(1-\theta)}^{N_0}$ \\ \\
	   
	    $\textbf{Take log on both sides}$ \\ \\
	    $log p(D/ \theta) = N_1 log \theta + N_0 log (1 - \theta)$ \\ \\
 $\textbf{Partially differentiate and equation to 0 to find maxima}$ \\ \\
 $\mathbf{\frac{N_1}{\widehat{\theta}}+ \frac{N_0}{1 - \widehat{\theta}} = 0 }$ \\ \\
 
  $\mathbf{\frac{N_1(1-\widehat{\theta})+N_0\widehat{\theta}}{\widehat{\theta}(1-\widehat{\theta})} = 0 }$ \\ \\
 $\textbf{Rearrange the terms to have theta in one side}$ \\ \\
 $ \mathbf{\widehat{\theta} = \frac{N_1}{N_1+N_0}}$ \\ \\
 
    \item 
    $ P(\theta)$ $\alpha$  $\theta^{\alpha}(1-\theta)^{\alpha}$ \\ \\
    $ P(\theta)$ $=$  $K\theta^{\alpha}(1-\theta)^{\alpha}$         $--(1)$ \\ \\
    $P(\theta|D) = \frac{P(D|\theta).P(\theta)}{P(D)}$ \\ \\
    \textbf{Take log on both sides} \\ \\
    $log P(\theta|D) $ = $log P(D|\theta) + log P(\theta) - log P(D)$ \\ \\
    \textbf{Put (1) in the previous equation} \\ \\
                      $ = N_1 log \theta + N_0 log (1-\theta) + \alpha log \theta + \alpha log (1-\theta)$ \\ \\
     \textbf{Partially differentiate the equation to 0 to find maxima}
     \\                   \\  
    $= \frac{N_1}{\theta} + \frac{N_0}{(1-\theta)} + \frac{\alpha}{\theta} + \frac{\alpha}{1-\theta}$    \\ \\
    \textbf{Rearrange with theta at LHS} \\ \\
    $\theta = \frac{N_1+\alpha}{N_1+N_0+2\alpha}$
    
 
 
	\end{enumerate}
\end{enumerate}
    
\end{document}

